state ext_spec for MMIO, but before I could prove compile_ext_call_correct for it, universe polymorphism errors stroke back, which might be resolved for the moment, but now MachineWidth creeps into this file, and letting it in does not work well, but rejecting it will require to remove it everywhere except in core riscv-coq

compiler/src/FlatToRiscvDef.v
@@ -18,9 +18,12 @@ Local Open Scope Z_scope.
 
 Set Implicit Arguments.
 
+Definition Register: Type := Z.
+(*Inductive EmptyType: Type :=.*)
+
 Module Import FlatToRiscvDef.
   Class parameters := {
-    actname: Set;
+    actname: Type;
     LwXLEN: Register -> Register -> Z -> Instruction;
     SwXLEN: Register -> Register -> Z -> Instruction;
     compile_ext_call: list Register -> actname -> list Register -> list Instruction;
@@ -28,7 +31,6 @@ Module Import FlatToRiscvDef.
     max_ext_call_code_size_nonneg: forall a, 0 <= max_ext_call_code_size a;
   }.
 End FlatToRiscvDef.
-
 
 Section FlatToRiscv1.
   Context {p: unique! FlatToRiscvDef.parameters}.
